fstar-helpers/fstar-bitvec/BitVec.Utils.fst
@@ -57,3 +57,11 @@ let forall256: forall_sig 256 = fun pred -> forall128 pred && forall128 (fun i -
 #pop-options
 
 let forall_n (n:nat{n <= 256}): forall_sig n = fun pred -> forall256 (fun i -> if i < n then pred i else true)
+
+let bit_vec_to_int_t_lemma
+    #t (d: num_bits t) (bv: bit_vec d)
+    i
+  : Lemma (get_bit (bit_vec_to_int_t d bv) (sz i) == bv i)
+          [SMTPat (get_bit (bit_vec_to_int_t d bv) (sz i))]
+  = bit_vec_to_int_t_lemma d bv i
+
